proofs/fstar/extraction-edited/Libcrux.Kem.Kyber.Serialize.PartA.fsti
@@ -1,4 +1,4 @@
-module Libcrux.Kem.Kyber.Serialize
+module Libcrux.Kem.Kyber.Serialize.PartA
 #set-options "--fuel 0 --ifuel 1 --z3rlimit 15"
 open Core
 open FStar.Mul
